extract/src/Prelude0.hs
@@ -1,0 +1,17 @@
+module Prelude0 where
+
+import qualified Util.HString as HString
+import qualified Data.Char
+import qualified Data.Function
+import qualified Data.List
+import qualified Data.Maybe
+import qualified Data.Ratio
+import qualified Data.Word
+import qualified Prelude
+import qualified System.IO.Unsafe
+
+
+apply :: () -> () -> (a1 -> a2) -> a1 -> a2
+apply _ _ f =
+  f
+
