extract/src/State.hs
@@ -1,0 +1,101 @@
+{-# OPTIONS_GHC -cpp -XMagicHash #-}
+{- For Hugs, use the option -F"cpp -P -traditional" -}
+
+module State where
+
+import qualified Util.HString as HString
+import qualified Data.Char
+import qualified Data.Function
+import qualified Data.List
+import qualified Data.Maybe
+import qualified Data.Ratio
+import qualified Data.Word
+import qualified Prelude
+import qualified System.IO.Unsafe
+
+import qualified Applicative
+import qualified Functor
+import qualified Ltac
+import qualified Monad
+import qualified Prelude0
+import qualified Tuple
+
+#ifdef __GLASGOW_HASKELL__
+import qualified GHC.Base
+#if __GLASGOW_HASKELL__ >= 900
+import qualified GHC.Exts
+#endif
+#else
+-- HUGS
+import qualified IOExts
+#endif
+
+#ifdef __GLASGOW_HASKELL__
+type Any = GHC.Base.Any
+#else
+-- HUGS
+type Any = ()
+#endif
+
+__ :: any
+__ = Prelude.error "Logical or arity value used"
+
+type StateT s m a = s -> m
+
+getT :: () -> (Applicative.Applicative a1) -> () -> StateT a2 a1 a2
+getT _ h _ i =
+  Applicative.pure __ h __ ((,) i i)
+
+getsT :: () -> (Applicative.Applicative a1) -> () -> () -> (a2 -> a3) ->
+         StateT a2 a1 a3
+getsT _ h _ _ f s =
+  Applicative.pure __ h __ ((,) (f s) s)
+
+modifyT :: () -> (Applicative.Applicative a1) -> () -> (a2 -> a2) -> StateT
+           a2 a1 ()
+modifyT _ h _ f i =
+  Applicative.pure __ h __ ((,) () (f i))
+
+coq_StateT_Functor :: () -> () -> (Functor.Functor a2) -> Functor.Functor
+                      (StateT a1 a2 Any)
+coq_StateT_Functor _ _ h =
+  Functor.Build_Functor (\_ _ f x st ->
+    Functor.fmap __ h __ __ (Tuple.first __ __ f __) (x st))
+
+coq_StateT_ap :: () -> (Monad.Monad a1) -> () -> () -> () -> (StateT 
+                 a2 a1 (a3 -> a4)) -> (StateT a2 a1 a3) -> StateT a2 
+                 a1 a4
+coq_StateT_ap _ h _ _ _ f x st =
+  Monad.join __ h __
+    (Functor.fmap __ (Applicative.is_functor __ (Monad.is_applicative __ h))
+      __ __ (\z ->
+      case z of {
+       (,) f' st' ->
+        Functor.fmap __
+          (Applicative.is_functor __ (Monad.is_applicative __ h)) __ __
+          (Tuple.first __ __ f' __) (x st')}) (f st))
+
+coq_StateT_Applicative :: () -> (Monad.Monad a1) -> () ->
+                          Applicative.Applicative (StateT a2 a1 Any)
+coq_StateT_Applicative _ h _ =
+  Applicative.Build_Applicative
+    (coq_StateT_Functor __ __
+      (Applicative.is_functor __ (Monad.is_applicative __ h))) (\_ x st ->
+    Applicative.pure __ (Monad.is_applicative __ h) __ ((,) x st))
+    (coq_StateT_ap __ h __)
+
+coq_StateT_join :: () -> (Monad.Monad a1) -> () -> () -> (StateT a2 a1
+                   (StateT a2 a1 a3)) -> StateT a2 a1 a3
+coq_StateT_join _ h _ _ x =
+  Ltac.comp __ __ __
+    (Ltac.comp __ __ __ (Monad.join __ h __)
+      (Functor.fmap __
+        (Applicative.is_functor __ (Monad.is_applicative __ h)) __ __
+        (Tuple.curry __ __ __ (Prelude0.apply __ __)))) x
+
+coq_StateT_Monad :: () -> (Monad.Monad a1) -> () -> Monad.Monad
+                    (StateT a2 a1 Any)
+coq_StateT_Monad _ h _ =
+  Monad.Build_Monad (coq_StateT_Applicative __ h __)
+    (coq_StateT_join __ h __)
+
