src/Lang.v
@@ -1,8 +1,9 @@
 Require Import
   Hask.Control.Monad
+  Hask.Control.Monad.Trans.State
   Hask.Control.Lens
   Pact.Data.Monoid
-  Pact.Data.RWSE
+  Pact.Data.Either
   Pact.Lib
   Pact.Ty
   Pact.Exp
@@ -36,34 +37,11 @@ Inductive EvalContext : Set :=
 
 Derive NoConfusion NoConfusionHom Subterm EqDec for EvalContext.
 
-Record PactEnv : Type := {
-  (* We cannot refer to capability tokens by their type here, because
-     capability predicates execute in a state monad that reference this
-     record type. *)
+Record PactState : Type := {
+  (* Read-only part of the state. *)
   _granted : list ACap;
   _context : list EvalContext;
-}.
 
-Derive NoConfusion NoConfusionHom Subterm EqDec for PactEnv.
-
-Definition newPactEnv : PactEnv :=
-  {| _granted := []
-   ; _context := []
-   |}.
-
-Definition granted : Lens' PactEnv (list ACap) :=
-  λ _ _ f env,
-    f (_granted env) <&> λ g,
-      {| _granted := g
-       ; _context := _context env |}.
-
-Definition context : Lens' PactEnv (list EvalContext) :=
-  λ _ _ f env,
-    f (_context env) <&> λ c,
-      {| _granted := _granted env
-       ; _context := c |}.
-
-Record PactState : Type := {
   (* We cannot refer to capability tokens by their type here, because
      capability predicates execute in a state monad that reference this
      record type. *)
@@ -74,54 +52,66 @@ Record PactState : Type := {
 Derive NoConfusion NoConfusionHom Subterm EqDec for PactState.
 
 Definition newPactState : PactState :=
-  {| _resources  := []
+  {| _granted    := []
+   ; _context    := []
+   ; _resources  := []
    ; _to_compose := []
    |}.
+
+Definition granted : Lens' PactState (list ACap) :=
+  λ _ _ f env,
+    f (_granted env) <&> λ g,
+      {| _granted    := g
+       ; _context    := _context env
+       ; _resources  := _resources env
+       ; _to_compose := _to_compose env
+       |}.
+
+Definition context : Lens' PactState (list EvalContext) :=
+  λ _ _ f env,
+    f (_context env) <&> λ c,
+      {| _granted    := _granted env
+       ; _context    := c
+       ; _resources  := _resources env
+       ; _to_compose := _to_compose env
+       |}.
 
 Definition resources : Lens' PactState (list ACap) :=
   λ _ _ f env,
     f (_resources env) <&> λ r,
-      {| _resources  := r
+      {| _granted    := _granted env
+       ; _context    := _context env
+       ; _resources  := r
        ; _to_compose := _to_compose env |}.
 
 Definition to_compose : Lens' PactState (list ACap) :=
   λ _ _ f env,
     f (_to_compose env) <&> λ tc,
-      {| _resources  := _resources env
+      {| _granted    := _granted env
+       ; _context    := _context env
+       ; _resources  := _resources env
        ; _to_compose := tc |}.
 
-Record PactLog : Set := MkLog {
-  entry : unit
-}.
+Definition PactM : Type → Type := @StateT PactState (Either Err).
 
-#[export]
-Program Instance PactLog_Semigroup : Semigroup PactLog := {|
-  mappend := λ '(MkLog _) '(MkLog _), MkLog tt
-|}.
+#[export] Instance PactM_Functor     : Functor PactM     := StateT_Functor.
+#[export] Instance PactM_Applicative : Applicative PactM := StateT_Applicative.
+#[export] Instance PactM_Monad       : Monad PactM       := StateT_Monad.
 
-#[export]
-Program Instance PactLog_SemigroupLaws : SemigroupLaws PactLog.
+Definition throw {a : Type} (err : Err) : PactM a := λ _, inl err.
 
-#[export]
-Program Instance PactLog_Monoid : Monoid PactLog := {|
-  mempty := MkLog tt
-|}.
+Definition localize `(l : Lens' PactState s) (f : s → s)
+  `(x : PactM a) : PactM a :=
+  s <- getsT (view l) ;
+  modifyT (set l (f s)) ;;
+  res <- x ;
+  modifyT (set l s) ;;
+  pure res.
 
-#[export]
-Program Instance PactLog_MonoidLaws : MonoidLaws PactLog.
-Next Obligation. sauto. Qed.
-Next Obligation. sauto. Qed.
-
-Derive NoConfusion NoConfusionHom Subterm EqDec for PactLog.
-
-Definition newPactLog : PactLog :=
-  MkLog tt.
-
-Definition PactM : Type → Type := @RWSE PactEnv PactLog PactState Err.
-
-#[export] Instance PactM_Functor     : Functor PactM     := RWSE_Functor.
-#[export] Instance PactM_Applicative : Applicative PactM := RWSE_Applicative.
-#[export] Instance PactM_Monad       : Monad PactM       := RWSE_Monad.
+Definition exchange `(l : Lens' PactState s) (st : s) : PactM s :=
+  s <- getsT (view l) ;
+  modifyT (set l st) ;;
+  pure s.
 
 Definition uncurryM `(f : a → PactM (b → PactM c)) : (a * b) → PactM c :=
   λ '(a, b), f' <- f a ; f' b.
@@ -135,12 +125,42 @@ Lemma uncurryM_curryM `(f : (a * b) → PactM c) :
 Proof.
   extensionality p.
   destruct p; simpl.
-  unfold RWSE_join.
-  rwse.
+  unfold StateT_join, Ltac.comp, Tuple.curry, Prelude.apply.
+  extensionality x.
   sauto lq: on.
 Qed.
 
 Lemma curryM_uncurryM `(f : a → PactM (b → PactM c)) :
   curryM (uncurryM f) = f.
 Proof.
+  unfold curryM, uncurryM.
+  extensionality p; simpl.
+  unfold StateT_join, Ltac.comp, Tuple.curry, Prelude.apply.
+  extensionality x.
+  simpl.
+  unfold Either_join, Either_map, curry, Tuple.first.
 Abort.
+
+Ltac unravel :=
+  repeat (cbv [
+    Datatypes.id
+    Either.Either_map
+    Lens.over
+    Lens.view
+    Lens.set
+    StateT_join
+    Either_join
+    Either_map
+    Tuple.first
+    Tuple.curry
+    granted
+    localize
+    Prelude.apply
+    exchange
+    getT
+    getsT
+    modifyT
+    putT
+    stepdownl'
+    Ltac.comp
+  ] in *; simpl in * ).
