src/Effects/Comp.v
@@ -1,0 +1,71 @@
+Require Import
+  Hask.Control.Monad.
+
+Generalizable All Variables.
+Set Primitive Projections.
+
+Definition Comp (A : Type) := A -> Prop.
+
+#[export]
+Program Instance Comp_Functor : Functor Comp := {
+  fmap := fun A B f (x : Comp A) b => exists a : A, x a /\ f a = b
+}.
+
+#[export]
+Program Instance Comp_Applicative : Applicative Comp := {
+  pure := fun _ x a => x = a;
+  ap   := fun A B mf mx r => exists f x, mf f /\ mx x /\ f x = r
+}.
+
+#[export]
+Program Instance Comp_Alternative : Alternative Comp := {
+  empty  := fun A _ => False;
+  choose := fun A x y s => x s \/ y s (* jww (2016-01-28): right? *)
+}.
+
+#[export]
+Program Instance Comp_Monad : Monad Comp := {
+  join := fun A m r => exists t : Comp A, t r /\ m t
+}.
+
+Require Import FunctionalExtensionality.
+
+Module CompLaws.
+
+Import MonadLaws.
+
+Axiom prop_ext : forall (P Q : Prop), (P <-> Q) -> P = Q.
+
+Ltac shatter :=
+  unfold comp, id in *;
+  repeat
+    match goal with
+    | [ H : _ = _           |- _               ] => subst
+    | [ H : and _ _         |- _               ] => destruct H
+    | [ H : exists _ : _, _ |- _               ] => destruct H
+    | [                     |- exists _ : _, _ ] => eexists
+    | [                     |- and _ _         ] => split
+    end;
+  simpl in *.
+
+Ltac simplify_comp :=
+  repeat let x := fresh "x" in extensionality x;
+  try (apply prop_ext; split; intros);
+  repeat (simpl; shatter; try constructor; eauto).
+
+Local Obligation Tactic := simpl; intros; simplify_comp.
+
+#[export]
+Program Instance Comp_FunctorLaws     : FunctorLaws Comp.
+#[export]
+Program Instance Comp_ApplicativeLaws : ApplicativeLaws Comp.
+#[export]
+Program Instance Comp_MonadLaws       : MonadLaws Comp.
+
+End CompLaws.
+
+Definition comp `(f : A -> Prop) : Comp A := f.
+
+Definition computes_to {A : Type} (ca : Comp A) (a : A) : Prop := ca a.
+
+Notation "c ↝ v" := (computes_to c v) (at level 40).
