src/Effects/Eff.v
@@ -1,0 +1,169 @@
+Require Import
+  Coq.Lists.List
+  Hask.Control.Monad.
+
+Require Export
+  Freer
+  Member.
+
+Import ListNotations.
+Import EqNotations.
+
+Generalizable All Variables.
+Set Primitive Projections.
+
+Definition sendF `(t : f a) : Freer f a := Impure t Pure.
+
+Definition Eff (effs : list (Type -> Type)) (a : Type) : Type :=
+  Freer (Union effs) a.
+
+Definition Arr effs a b := a -> Eff effs b.
+Arguments Arr effs a b /.
+
+Definition send `{Member eff effs} `(t : eff a) : Eff effs a :=
+  Impure (inj t) Pure.
+
+#[export]
+Instance Functor_Eff {r} : Functor (Eff r) := Freer_Functor _.
+#[export]
+Instance Applicative_Eff {r} : Applicative (Eff r) := Freer_Applicative _.
+#[export]
+Instance Monad_Eff {r} : Monad (Eff r) := Freer_Monad _.
+
+Definition run `(f : Eff [] a) : a :=
+  match f with
+  | Pure x => x
+  | Impure u k => False_rect _ ltac:(inversion u)
+  end.
+
+Fixpoint runM `{Monad m} `(f : Eff [m] a) : m a :=
+  match f with
+  | Pure x     => pure x
+  | Impure u q => extract u >>= (runM \o q)
+  end.
+
+Fixpoint handleRelay
+  `(ret : a -> Eff effs b)
+  `(bind : forall v, eff v -> Arr effs v b -> Eff effs b)
+  (f : Eff (eff :: effs) a) : Eff effs b :=
+  match f with
+  | Pure x => ret x
+  | Impure u q =>
+    let k := handleRelay ret bind \o q in
+    match decomp u with
+    | inl x => bind _ x k
+    | inr u => Impure u k
+    end
+  end.
+
+Fixpoint handleRelayS
+  `(st : s)
+  `(ret : s -> a -> Eff effs b)
+  `(bind : forall v, s -> eff v -> (s -> Arr effs v b) -> Eff effs b)
+  (f : Eff (eff :: effs) a) : Eff effs b :=
+  match f with
+  | Pure x => ret st x
+  | Impure u q =>
+    let k st' := handleRelayS st' ret bind \o q in
+    match decomp u with
+    | inl x => bind _ st x k
+    | inr u => Impure u (k st)
+    end
+  end.
+
+Fixpoint replaceRelay
+  `(ret : a -> Eff (v :: effs) b)
+  `(bind : forall x, t x -> Arr (v :: effs) x b -> Eff (v :: effs) b)
+  (f : Eff (t :: effs) a) :
+  Eff (v :: effs) b :=
+  match f with
+  | Pure x => ret x
+  | Impure u q =>
+    let k := replaceRelay ret bind \o q in
+    match decomp u with
+    | inl x => bind _ x k
+    | inr u => Impure (weaken u) k
+    end
+  end.
+
+Fixpoint replaceRelayN
+  `{Weakens gs}
+  `(pure' : a -> Eff (gs ++ effs) w)
+  `(bind : forall x, t x -> Arr (gs ++ effs) x w -> Eff (gs ++ effs) w)
+  (f : Eff (t :: effs) a) :
+  Eff (gs ++ effs) w :=
+  match f with
+  | Pure x => pure' x
+  | Impure u q =>
+    let k := replaceRelayN pure' bind \o q in
+    match decomp u with
+    | inl x => bind _ x k
+    | inr u => Impure (weakens u) k
+    end
+  end.
+
+Definition interpretWith
+  `(bind : forall v, eff v -> Arr effs v a -> Eff effs a) :
+  Eff (eff :: effs) a -> Eff effs a := handleRelay Pure bind.
+
+Definition interpret `(handler : eff ~> Eff effs) :
+  Eff (eff :: effs) ~> Eff effs :=
+  fun _ => interpretWith (fun _ e f => handler _ e >>= f).
+
+Fixpoint handleInterpose {eff effs a b}
+         `{M : Member eff effs}
+         (ret : a -> Eff effs b)
+         (bind : forall v, eff v -> Arr effs v b -> Eff effs b)
+         (f : Eff effs a) : Eff effs b :=
+  match f with
+  | Pure x => ret x
+  | Impure u q =>
+    let k := handleInterpose ret bind \o q in
+    match @prj eff effs M _ u with
+    | Some x => bind _ x k
+    | None   => Impure u k
+    end
+  end.
+
+Definition interposeWith `{Member eff effs}
+  `(bind : forall v, eff v -> Arr effs v a -> Eff effs a) :
+  Eff effs a -> Eff effs a := handleInterpose Pure bind.
+
+Definition interpose `{Member eff effs} `(handler : eff ~> Eff effs) :
+  Eff effs ~> Eff effs :=
+  fun _ => interposeWith (fun _ e f => handler _ e >>= f).
+
+Definition subsume `{Member eff effs} : Eff (eff :: effs) ~> Eff effs :=
+  interpret (fun _ => send).
+
+Definition reinterpret `(t : f ~> Eff (g :: effs)) :
+  Eff (f :: effs) ~> Eff (g :: effs) :=
+  fun _ => replaceRelay Pure (fun _ e f => t _ e >>= f).
+
+Definition reinterpretN `{Weakens gs}
+  `(k : f ~> Eff (gs ++ effs)) : Eff (f :: effs) ~> Eff (gs ++ effs) :=
+  fun _ => replaceRelayN Pure (fun _ e f => k _ e >>= f).
+
+Definition reinterpret2
+  `(k : f ~> Eff (g :: h :: effs)) : Eff (f :: effs) ~> Eff (g :: h :: effs) :=
+  reinterpretN (gs:=[g; h]) k.
+
+Definition reinterpret3
+  `(k : f ~> Eff (g :: h :: i :: effs)) :
+  Eff (f :: effs) ~> Eff (g :: h :: i :: effs) :=
+  reinterpretN (gs:=[g; h; i]) k.
+
+Definition translate `(t : f ~> g) {effs} : Eff (f :: effs) ~> Eff (g :: effs) :=
+  reinterpret (fun _ => send \o t _).
+
+Definition extrude {f effs} : Eff (f :: effs) ~> Eff (f :: f :: effs) :=
+  reinterpret2 (fun _ => send \o id).
+
+Fixpoint raise {e} `(f : Eff effs a) : Eff (e :: effs) a :=
+  match f with
+  | Pure x => Pure x
+  | Impure u k => Impure (weaken u) (fun x => raise (k x))
+  end.
+
+Definition composed {f g h : Type -> Type}
+  `(y : g ~> h) `(x : f ~> g) : f ~> h := fun _ => y _ \o x _.
