src/Effects/Freer.v
@@ -1,0 +1,265 @@
+Require Import
+  FunctionalExtensionality
+  Hask.Control.Monad.
+
+Generalizable All Variables.
+
+Inductive Fix (f : Type -> Type) : Type :=
+  | mkFix : forall x, f x -> (x -> Fix f) -> Fix f.
+
+Arguments mkFix {f x} _ _.
+
+Definition Freer' (f : Type -> Type) (a : Type) : Type :=
+  Fix (fun t => a + f t)%type.
+
+Inductive Freer (f : Type -> Type) (a : Type) : Type :=
+  | Pure : a -> Freer f a
+  | Impure : forall x, f x -> (x -> Freer f a) -> Freer f a.
+
+Arguments Pure {f a} _.
+Arguments Impure {f a x} _ _.
+
+Fixpoint toFreer `(x : Freer' f a) : Freer f a :=
+  match x with
+  | mkFix (inl a) _ => Pure a
+  | mkFix (inr u) k => Impure u (toFreer \o k)
+  end.
+
+Fixpoint fromFreer `(x : Freer f a) : Freer' f a :=
+  match x with
+  | Pure a     => mkFix (x:=False) (inl a) (False_rect _)
+  | Impure u k => mkFix (inr u) (fromFreer \o k)
+  end.
+
+Theorem fromFreer_toFreer `(x : Freer' f a) : fromFreer (toFreer x) = x.
+Proof.
+  induction x; simpl in *.
+  destruct f0; simpl.
+    (* [Freer] is "bigger" than [Freer'], since it contains information about
+       the existential type (and a mapping from it) even in the terminating
+       case. *)
+    assert (x = False) by admit.
+    subst.
+    f_equal.
+    extensionality z.
+    contradiction.
+  f_equal.
+  unfold comp.
+  extensionality z.
+  apply H.
+Admitted.
+
+Theorem toFreer_fromFreer `(x : Freer f a) : toFreer (fromFreer x) = x.
+Proof.
+  induction x; simpl in *; auto.
+  f_equal.
+  unfold comp.
+  extensionality z.
+  apply H.
+Qed.
+
+Fixpoint Freer_map {r} `(f : a -> b) (x : Freer r a) : Freer r b :=
+  match x with
+  | Pure v => Pure (f v)
+  | Impure u k => Impure u (fun x => Freer_map f (k x))
+  end.
+
+#[export]
+Program Instance Freer_Functor (f : Type -> Type) : Functor (Freer f) := {
+  fmap := @Freer_map _
+}.
+
+Fixpoint Freer_ap {r} `(f : Freer r (a -> b)) (x : Freer r a) : Freer r b :=
+  match f, x with
+  | Pure f, Pure v     => Pure (f v)
+  | Pure f, Impure u k => Impure u (fun x => Freer_map f (k x))
+  | Impure u k, m      => Impure u (fun x => Freer_ap (k x) m)
+  end.
+
+#[export]
+Program Instance Freer_Applicative (f : Type -> Type) : Applicative (Freer f) := {
+  pure := fun _ => Pure;
+  ap := fun _ _ => Freer_ap
+}.
+
+Fixpoint Freer_join {r} `(f : Freer r (Freer r a)) : Freer r a :=
+  match f with
+  | Pure v     => v
+  | Impure u k => Impure u (fun x => Freer_join (k x))
+  end.
+
+#[export]
+Program Instance Freer_Monad (f : Type -> Type) : Monad (Freer f) := {
+  join := @Freer_join _
+}.
+
+Module FreerLaws.
+
+Include MonadLaws.
+
+#[export]
+Program Instance Freer_FunctorLaws (f : Type -> Type) : FunctorLaws (Freer f).
+Next Obligation.
+  extensionality x.
+  induction x; simpl; auto.
+  unfold id.
+  f_equal; simpl.
+  extensionality y.
+  apply H.
+Qed.
+Next Obligation.
+  extensionality x.
+  induction x; simpl; auto.
+  unfold comp.
+  f_equal; simpl.
+  extensionality y.
+  apply H.
+Qed.
+
+#[export]
+Program Instance Freer_ApplicativeLaws (f : Type -> Type) : ApplicativeLaws (Freer f).
+Next Obligation.
+  extensionality x.
+  induction x;
+  unfold Freer_map, comp; simpl; auto.
+  unfold id.
+  f_equal.
+  extensionality y.
+  specialize (H y).
+  destruct (f1 y); auto.
+Qed.
+Next Obligation.
+  unfold Freer_ap, Freer_map, comp; simpl; auto.
+  induction u, v, w; simpl; auto;
+  f_equal;
+  extensionality y; simpl;
+  try (specialize (H y);
+       destruct (f1 y); auto).
+  - induction (f1 y); auto.
+    f_equal.
+    extensionality z; simpl.
+    specialize (H z).
+    destruct (f3 z); auto.
+  - induction (f1 y); auto.
+    f_equal.
+    extensionality z; simpl.
+    specialize (H z).
+    destruct (f3 z); auto.
+  - induction (f1 y); auto.
+      f_equal.
+      extensionality z; simpl.
+      induction (f3 z); auto.
+      f_equal.
+      extensionality w; simpl.
+      specialize (H w).
+      destruct (f5 w); auto.
+    f_equal.
+    extensionality z; simpl.
+    specialize (H z).
+    destruct (f5 z); auto.
+Qed.
+Next Obligation.
+  unfold Freer_ap, Freer_map, comp; simpl; auto.
+  induction u; auto.
+  f_equal.
+  extensionality x0.
+  specialize (H x0).
+  destruct (f1 x0); auto.
+Qed.
+Next Obligation.
+  unfold Freer_ap, Freer_map, comp; simpl; auto.
+  extensionality x0.
+  destruct x0; auto.
+Qed.
+
+#[export]
+Program Instance Freer_MonadLaws (f : Type -> Type) : MonadLaws (Freer f).
+Next Obligation.
+  extensionality x.
+  induction x;
+  unfold Freer_join, Freer_map, comp; simpl; auto.
+  f_equal.
+  extensionality y.
+  apply H.
+Qed.
+Next Obligation.
+  extensionality x.
+  induction x;
+  unfold Freer_join, Freer_map, comp; simpl; auto.
+  unfold id.
+  f_equal.
+  extensionality y.
+  apply H.
+Qed.
+Next Obligation.
+  extensionality x.
+  induction x;
+  unfold Freer_join, Freer_map, comp; simpl; auto.
+  unfold id.
+  f_equal.
+  extensionality y.
+  apply H.
+Qed.
+
+End FreerLaws.
+
+Fixpoint iter `{Functor f} `(phi : f a -> a) (fr : Freer f a) : a :=
+  match fr with
+    | Pure x => x
+    | Impure h g => phi (fmap (iter phi \o g) h)
+  end.
+
+Inductive iterP `{Functor f} `(phi : f a -> a -> Prop) :
+  Freer f a -> a -> Prop :=
+  | IterPure : forall x,
+      iterP phi (Pure x) x
+  | IterImpure : forall h g x r,
+      phi h x ->
+      iterP phi (g x) r ->
+      iterP phi (Impure h g) r.
+
+Definition liftF {f : Type -> Type} {a : Type} : f a -> Freer f a :=
+  fun x => Impure x Pure.
+
+Definition uniter `{Functor f} `(psi : Freer f a -> a) : f a -> a :=
+  psi \o liftF.
+
+Fixpoint retract `{Monad f} `(fr : Freer f a) : f a :=
+  match fr with
+    | Pure x => pure x
+    | Impure h g => h >>= (retract \o g)
+  end.
+
+Fixpoint hoistFree `(n : forall a, f a -> g a) `(fr : Freer f b) : Freer g b :=
+  match fr with
+  | Pure x => Pure x
+  | Impure h g => Impure (n _ h) (hoistFree n \o g)
+  end.
+
+Fixpoint foldFree `{Monad m} `(n : forall x, f x -> m x) `(fr : Freer f a) :
+  m a :=
+  match fr with
+  | Pure x => pure x
+  | Impure h g => join (fmap (foldFree n \o g) (n _ h))
+  end.
+
+(*
+Inductive foldFreeP `{Monad m} `(phi : forall x, f x -> m x -> Prop) {a} :
+  Freer f a -> m a -> Prop :=
+  | FoldPure : forall x,
+      foldFreeP phi (Pure x) (pure x)
+  | FoldImpure : forall t h g x r,
+      phi t h x ->
+      foldFreeP phi (x >>= g) r ->
+      foldFreeP phi (Impure (x:=t) h g) r.
+*)
+
+Fixpoint cutoff (n : nat) `(fr : Freer f a) : Freer f (option a) :=
+  match n with
+  | O => Pure None
+  | S n' =>
+    match fr with
+    | Pure x => Pure (Some x)
+    | Impure h g => Impure h (cutoff n \o g)
+    end
+  end.
