src/Effects/Fused.v
@@ -1,0 +1,409 @@
+Require Export Hask.Control.Monad.
+Require Import Hask.Control.Monad.Trans.Reader.
+Require Import Hask.Control.Monad.State.
+Require Import Hask.Control.Monad.Trans.State.
+Require Import Pact.Data.Either.
+Require Import Hask.Control.Compose.
+
+Require Export Equations.Prop.DepElim.
+From Equations Require Export Equations.
+
+Set Universe Polymorphism.
+Generalizable All Variables.
+
+#[export]
+Program Instance id_Functor : Functor id := {|
+  fmap := fun _ _ f x => f x
+|}.
+#[export]
+Program Instance id_Applicative : Applicative id := {|
+  pure := fun _ x => x;
+  ap := fun _ _ f x => f x
+|}.
+#[export]
+Program Instance id_Monad : Monad id.
+
+#[export]
+Program Instance arrow_Functor {r} : Functor (fun a => r -> a) := {|
+  fmap := fun _ _ f x r => f (x r)
+|}.
+#[export]
+Program Instance arrow_Applicative {r} : Applicative (fun a => r -> a) := {|
+  pure := fun _ x _ => x;
+  ap := fun _ _ f x r => f r (x r)
+|}.
+#[export]
+Program Instance arrow_Monad {r} : Monad (fun a => r -> a) := {|
+  join := fun _ x r => x r r
+|}.
+
+Definition Handler ctx (m n : Type -> Type) :=
+  forall x, ctx (m x) -> n (ctx x).
+
+Definition hcomp `{Functor n} `{Functor ctx1} {ctx2 l m}
+  (hdl1 : Handler ctx1 m n) (hdl2 : Handler ctx2 l m) :
+  Handler (ctx1 \o ctx2) l n :=
+  fun _ => hdl1 _ \o fmap (hdl2 _).
+
+Infix "~<~" := hcomp (at level 51, right associativity).
+
+Definition Sig : Type := (Type -> Type) -> (Type -> Type).
+
+Inductive Sum (f g : Sig) (m : Type -> Type) : Type -> Type :=
+  | L {k} : f m k -> Sum f g m k
+  | R {k} : g m k -> Sum f g m k.
+
+Infix ":+:" := Sum (at level 51, right associativity).
+
+Arguments L {_ _ _ k} _.
+Arguments R {_ _ _ k} _.
+
+Equations reassociateSumL `(s : (l1 :+: l2 :+: r) m a) :
+  ((l1 :+: l2) :+: r) m a :=
+  reassociateSumL (L l)     := L (L l);
+  reassociateSumL (R (L l)) := L (R l);
+  reassociateSumL (R (R x)) := R x.
+
+Class Algebra (sg : Sig) (m : Type -> Type) `{Monad m} := {
+  alg `{Functor ctx} {n a}
+    : Handler ctx n m
+    -> sg n a
+    -> ctx unit
+    -> m (ctx a)
+}.
+
+Close Scope nat_scope.
+
+Class Member (sub sup : Sig) := {
+  inj {m a} : sub m a -> sup m a
+}.
+
+#[export]
+Instance Member_assoc {t l1 l2 r} :
+  Member t (l1 :+: l2 :+: r) -> Member t ((l1 :+: l2) :+: r) | 9 := fun _ => {|
+  inj := fun _ _ => reassociateSumL \o inj
+|}.
+
+#[export]
+Instance Member_tl {l l' r} : Member l r -> Member l (l' :+: r) | 3 := fun _ => {|
+  inj := fun _ _ => R \o inj
+|}.
+
+#[export]
+Instance Member_hd {l r} : Member l (l :+: r) | 2 := {|
+  inj := fun _ _ => L
+|}.
+
+#[export]
+Instance Member_refl {t} : Member t t | 1 := {|
+  inj := fun _ _ => id
+|}.
+
+Class Members (sub sup : Sig) := {
+  membership : Member sub sup
+}.
+
+#[export] Program Instance is_Member {t u} : Member t u -> Members t u | 2.
+
+#[export] Program Instance sum_Members {l r u} :
+  Members l u -> Members r u -> Members (l :+: r) u | 1.
+Next Obligation.
+  constructor; intros.
+  destruct X.
+  - now apply H.
+  - now apply H0.
+Defined.
+
+(* Definition Has eff sig m `{Monad m} : Type := Members eff sig * Algebra sig m. *)
+
+Definition Has (eff sg : Sig) (m : Type -> Type)
+  `{M : Monad m} `{U : Members eff sg} `{A : Algebra sg m (H:=M)} := True.
+
+Definition send `{Member eff sg} `{A : Algebra sg m} `(f : eff m a) : m a :=
+  alg (Algebra:=A) (H0:=id_Functor) (fun _ x => ltac:(eexact x)) (inj f) tt.
+
+Inductive Throw e (m : Type -> Type) (a : Type) : Type :=
+  | Raise : e -> Throw e m a.
+
+Arguments Raise {_ _ _} _.
+
+Inductive Catch e (m : Type -> Type) (a : Type) : Type :=
+  | Handle : m a -> (e -> m a) -> Catch e m a.
+
+Arguments Handle {_ _ _} _ _.
+
+Definition Error e := Throw e :+: Catch e.
+
+Definition errorAlg {e} `{Functor ctx} {n a}
+  (hdl : Handler ctx n (Either e))
+  (s : Error e n a)
+  (u : ctx unit) : Either e (ctx a) :=
+  match s with
+  | L (Raise e)    => Left e
+  | R (Handle m h) =>
+      either (hdl _ \o (fun x => x <$ u) \o h) pure (hdl _ (m <$ u))
+  end.
+
+#[export]
+Instance Error_Algebra {e} : Algebra (Error e) (Either e) := {|
+  alg := @errorAlg e
+|}.
+
+Inductive Reader r (m : Type -> Type) : Type -> Type :=
+  | Ask       :                    Reader r m r
+  | Local {a} : (r -> r) -> m a -> Reader r m a.
+
+Arguments Ask {_ _}.
+Arguments Local {_ _ _} _ _.
+
+Definition readerAlg {r} `{Functor ctx} {n a}
+  (hdl : Handler ctx n (fun a => r -> a))
+  (s : Reader r n a)
+  (u : ctx unit) : r -> ctx a :=
+  match s with
+  | Ask       => fun x => x <$ u
+  | Local f m => hdl _ (m <$ u) \o f
+  end.
+
+#[export]
+Program Instance Reader_Algebra {r} : Algebra (Reader r) (fun a => r -> a) := {|
+  alg := @readerAlg r
+|}.
+
+Definition asksT `(f : r -> a) `{Monad m} : ReaderT r m a :=
+  fun r => pure (f r).
+
+Definition localT `(f : r -> r) `(x : ReaderT r m a) : ReaderT r m a :=
+  fun r => x (f r).
+
+Equations readerTAlg {r sig m} `{Monad m} `{Algebra sig m} `{Functor ctx} {n a}
+  (hdl : Handler ctx n (ReaderT r m))
+  (s : (Reader r :+: sig) n a)
+  (u : ctx unit) : ReaderT r m (ctx a) :=
+  readerTAlg hdl (L Ask) u :=
+    asksT (fun x => x <$ u);
+  readerTAlg hdl (L (Local f mo)) u :=
+    localT f (hdl _ (mo <$ u));
+  readerTAlg hdl (R other) u :=
+    fun r => alg (fun x => (fun f => f r) \o hdl x) other u.
+
+#[export]
+Instance ReaderT_Algebra {r sig m} `{Monad m} :
+  Algebra sig m -> Algebra (Reader r :+: sig) (ReaderT r m) := fun H => {|
+  alg := @readerTAlg r _ _ _ _ H
+|}.
+
+Section Reader.
+
+Context `{Member (Reader r) sg}.
+Context `{Algebra sg m}.
+
+Definition ask : m r := send Ask.
+
+Definition local (f : r -> r) `(x : m a) : m a :=
+  send (Local f x).
+
+End Reader.
+
+(************************************************************************)
+
+Inductive State s (m : Type -> Type) : Type -> Type :=
+  | Get :      State s m s
+  | Put : s -> State s m unit.
+
+Arguments Get {_ _}.
+Arguments Put {_ _} _.
+
+Definition stateAlg {s} `{Functor ctx} {n a}
+  (hdl : Handler ctx n (State.State s))
+  (sg : State s n a)
+  (u : ctx unit) : State.State s (ctx a) :=
+  match sg with
+  | Get   => fun s => (s <$ u, s)
+  | Put m => fun _ => (u, m)
+  end.
+
+#[export]
+Instance State_Algebra {s} : Algebra (State s) (State.State s) := {|
+  alg := @stateAlg s
+|}.
+
+Definition getsT `(f : s -> a) `{Monad m} : StateT s m a :=
+  fun s => pure (f s, s).
+
+Definition putT `(x : s) `{Monad m} : StateT s m unit :=
+  fun _ => pure (tt, x).
+
+Definition thread `{Functor ctx1} `{Functor ctx2}
+  `{Algebra sg m} {n a} :
+     Handler (ctx1 \o ctx2) n m
+  -> sg n a
+  -> ctx1 (ctx2 unit)
+  -> m (ctx1 (ctx2 a)) :=
+  fun hdl s => alg hdl s.
+
+#[local] Remove Hints Compose_Alternative : typeclass_instances.
+
+#[export]
+Instance Tuple_Functor {S} : Functor (fun a => (a * S)%type) | 9 := {
+  fmap := fun _ _ f p => (f (fst p), snd p)
+}.
+
+Equations stateTAlg {s sig m} `{Monad m} `{Algebra sig m} `{Functor ctx} {n a}
+  (hdl : Handler ctx n (StateT s m))
+  (sg : (State s :+: sig) n a)
+  (u : ctx unit) : StateT s m (ctx a) :=
+  stateTAlg hdl (L Get) u     := getsT (fun x => x <$ u);
+  stateTAlg hdl (L (Put x)) u := u <$ putT x;
+  stateTAlg hdl (R other) u   :=
+    fun st => thread (ctx1:=fun a => a * s)
+                ((fun _ '(f, s') => f s') ~<~ hdl) other (u, st).
+
+#[export]
+Instance StateT_Algebra {s sig m} `{Monad m} :
+  Algebra sig m -> Algebra (State s :+: sig) (StateT s m) := fun H => {|
+  alg := @stateTAlg s _ _ _ _ H
+|}.
+
+Section State.
+
+Context `{Member (State s) sg}.
+Context `{Algebra sg m}.
+
+Definition get : m s := send Get.
+
+Definition gets `(f : s -> a) : m a := f <$> get.
+
+Definition put : s -> m unit := send \o Put.
+
+Definition modify (f : s -> s) : m unit := get >>= (put \o f).
+
+Definition state `(f : s -> (s * a)) : m a :=
+  p <- gets f ;
+  let '(s', a) := p in
+  a <$ put s'.
+
+End State.
+
+Definition sample
+  `{Member (State nat) sg}
+  `{Member (Reader bool) sg}
+  `{Algebra sg m} : m unit :=
+  b <- ask ;
+  if b : bool
+  then
+    n <- get ;
+    put (n + 10)%nat
+  else
+    put 100%nat.
+
+Definition runReader `(env : r) `(x : r -> a) : a := x env.
+Definition runReaderT `(env : r) `(x : ReaderT r m a) : m a := x env.
+
+Definition runState `(st : s) `(x : State.State s a) : a * s := x st.
+Definition runStateT `(st : s) `(x : StateT s m a) : m (a * s) := x st.
+
+(* This uses the StateT carrier. *)
+Definition example1 `{Algebra sg m} : m (unit * nat) :=
+  runReaderT true (runStateT 0%nat sample).
+
+(* This uses the State carrier. No final [run] is needed, because in Coq the
+  Identity monad is the [id] function, so [run x = x]. *)
+Definition example2 : unit * nat :=
+  runReader true (runStateT 0%nat sample).
+
+(************************************************************************)
+
+Require Import Hask.Control.Lens.
+Require Import Pact.Data.Monoid.
+
+Program Definition focus `(l : Lens' s s')
+  `{Member (State s) sg} `{A : Algebra sg m}
+  `(f : forall `{Member (State s') sg}, m a) : m a :=
+  @f _.
+Next Obligation.
+  constructor; intros.
+  induction X.
+  - apply inj.
+  - pose (st <- get ;
+           modify X0 ;;
+           res <- X1 ;
+           put st ;;
+           pure res).
+
+Program Definition readonly `(l : Lens' s r)
+  `{Member (State Foo) sg} `{A : Algebra sg m}
+  `(f : forall `{Member (Reader Foo) sg}, m a) : m a :=
+  @f _.
+Next Obligation.
+  constructor; intros.
+  apply inj.
+  inversion X; subst.
+  - exact (Get (m:=m0)).
+  - pose (st <- get ;
+           modify X0 ;;
+           res <- X1 ;
+           put st ;;
+           pure res).
+
+(*
+
+Definition appendonly `(l : Lens' s w) `{Monoid w} {effs} :
+  Eff (Writer w :: effs) ~> Eff (State s :: effs) :=
+  reinterpret (fun _ f =>
+    let '(a, w) := writerAlg f in
+    modify (over l (mappend w)) ;;
+    pure a).
+*)
+
+Definition overM `(l : Lens s t a b) `{Functor f} : (a -> f b) -> s -> f t := l f _.
+Notation "l %%~ f" := (overM l f) (at level 40).
+
+Polymorphic Inductive Foo : Type := mkFoo.
+Polymorphic Inductive Bar : Type := mkBar.
+Polymorphic Inductive Baz : Type := mkBaz.
+
+Record SomeState : Type := {
+  _foo : Foo;
+  _bar : Bar;
+  _baz : Baz;
+}.
+
+Definition foo : Lens' SomeState Foo :=
+  fun _ _ f env =>
+    f (_foo env) <&> fun g =>
+      {| _foo := g
+       ; _bar := _bar env
+       ; _baz := _baz env |}.
+
+Definition bar : Lens' SomeState Bar :=
+  fun _ _ f env =>
+    f (_bar env) <&> fun g =>
+      {| _foo := _foo env
+       ; _bar := g
+       ; _baz := _baz env |}.
+
+Definition baz : Lens' SomeState Baz :=
+  fun _ _ f env =>
+    f (_baz env) <&> fun g =>
+      {| _foo := _foo env
+       ; _bar := _bar env
+       ; _baz := g |}.
+
+Declare Instance Baz_Monoid : Monoid Baz.
+
+Definition sample3 `{Member (Reader Foo) sg} `{Algebra sg m} : m unit :=
+  pure tt.
+
+Definition sample4 `{Member (State Foo) sg} `{A : Algebra sg m} : m unit :=
+  @sample3 sg _ m _ A.
+
+Definition example3 : Eff [State SomeState] unit :=
+  subsume _
+    (focus baz _
+        (appendonly (fun _ _ => id) _
+           (subsume _
+              (focus bar _
+                 (subsume _
+                    (focus foo _
+                       (readonly (fun _ _ => id) _ sample))))))).
