src/Effects/Member.v
@@ -1,0 +1,65 @@
+Require Import
+  Coq.Lists.List.
+
+Require Export
+  Union.
+
+Import ListNotations.
+
+Generalizable All Variables.
+
+Inductive FindElem (t : Type -> Type) : list (Type -> Type) -> Type :=
+  | Here : forall xs, FindElem t (t :: xs)
+  | Next : forall t' xs, FindElem t xs -> FindElem t (t' :: xs).
+
+Class Member (t : Type -> Type) (r : list (Type -> Type)) := {
+  inj : forall v, t v -> Union r v;
+  prj : forall v, Union r v -> option (t v);
+  hasElem : FindElem t r
+}.
+
+Arguments inj {t r _ v} _.
+Arguments prj {t r _ v} _.
+
+#[export]
+Program Instance Member_Here (t : Type -> Type) (r : list (Type -> Type)) :
+  Member t (t :: r) | 1 := {
+  inj := fun _ x => UThis x;
+  prj := fun _ u =>
+    match decomp u with
+    | inl x => Some x
+    | inr _ => None
+    end;
+  hasElem := Here _ _
+}.
+
+#[export]
+Program Instance Member_Next (t t' : Type -> Type) (r : list (Type -> Type)) :
+  Member t r -> Member t (t' :: r) | 2 := {
+  inj := fun _ x => UThat (inj x);
+  prj := fun _ u =>
+    match decomp u with
+    | inl _ => None
+    | inr u => prj u
+    end;
+  hasElem := Next _ _ _ hasElem
+}.
+
+Fixpoint FindElem_last  (t : Type -> Type) (r : list (Type -> Type)) :
+  FindElem t (r ++ [t]) :=
+  match r with
+  | [] => Here _ _
+  | _ :: xs => Next _ _ _ (FindElem_last t xs)
+  end.
+
+#[export]
+Program Instance Member_Last (t : Type -> Type) (r : list (Type -> Type)) :
+  Member t (r ++ [t]) | 2 := {
+  inj := fun _ x => inject_last t r x;
+  prj := fun _ u =>
+    match decomp_rev u with
+    | inl _ => None
+    | inr x => Some x
+    end;
+  hasElem := FindElem_last t r
+}.
