src/Effects/RWS.v
@@ -1,0 +1,190 @@
+Require Import
+  Coq.Lists.List
+  Pact.Data.Monoid
+  Pact.Data.IList
+  Hask.Control.Monad.
+
+Require Export
+  Eff.
+
+Require Export Equations.Prop.DepElim.
+From Equations Require Export Equations.
+
+Import ListNotations.
+
+Generalizable All Variables.
+Set Primitive Projections.
+
+(************************************************************************)
+
+Polymorphic Inductive Reader (r : Type) : Type -> Type :=
+  | Ask : Reader r r.
+
+Arguments Ask {r}.
+
+Fixpoint runReader' `(x : e) `(f : Freer (Reader e) a) : a :=
+  match f with
+  | Pure v => v
+  | Impure Ask k => runReader' x (k x)
+  end.
+
+Definition ask {r effs} `{Member (Reader r) effs} : Eff effs r :=
+  send Ask.
+
+Definition asks {r effs a} `{Member (Reader r) effs} (f : r -> a) : Eff effs a :=
+  f <$> ask.
+
+Definition readerAlg `(x : r) `(f : Reader r a) : a :=
+  match f with Ask => x end.
+
+Definition local {r effs a} `{Member (Reader r) effs} (f : r -> r) (m : Eff effs a) :
+  Eff effs a :=
+  r <- asks f ;
+  interpose (fun _ => Pure \o readerAlg r) _ m.
+
+Definition runReader `(x : e) {r} : Eff (Reader e :: r) ~> Eff r :=
+  interpret (fun _ => Pure \o readerAlg x).
+
+(************************************************************************)
+
+Inductive Writer (w : Type) : Type -> Type :=
+  | Tell : w -> Writer w unit.
+
+Arguments Tell {w} _.
+
+Fixpoint runWriter' `{Monoid w} `(f : Freer (Writer w) a) : a * w :=
+  match f with
+  | Pure v => (v, mempty)
+  | Impure (Tell x) k =>
+      let '(v, l) := runWriter' (k tt) in (v, x ⨂ l)
+  end.
+
+Definition tell {w effs} `{Member (Writer w) effs} : w -> Eff effs unit :=
+  send \o Tell.
+
+Definition writerAlg `{Monoid w} `(f : Writer w a) : a * w :=
+  match f with Tell x => (tt, x) end.
+
+Definition second {A B C} (f : B -> C) (p : A * B) : A * C :=
+  (fst p, f (snd p)).
+
+Definition runWriter {w effs a} `{Monoid w} :
+  Eff (Writer w :: effs) a -> Eff effs (a * w) :=
+  handleRelay (fun x => Pure (x, mempty))
+    (fun _ w k => let '(a, w') := writerAlg w in second (mappend w') <$> k a).
+
+(************************************************************************)
+
+Inductive State (s : Type) : Type -> Type :=
+  | Get : State s s
+  | Put : s -> State s unit.
+
+Arguments Get {s}.
+Arguments Put {s} _.
+
+Fixpoint runState' `(f : Freer (State s) a) (st : s) : (a * s) :=
+  match f with
+  | Pure v => (v, st)
+  | Impure Get k =>
+      let '(v, s') := runState' (k st) st in (v, s')
+  | Impure (Put s) k =>
+      let '(v, s') := runState' (k tt) s in (v, s')
+  end.
+
+Definition get {s effs} `{Member (State s) effs} : Eff effs s :=
+  send Get.
+
+Definition put {s effs} `{Member (State s) effs} : s -> Eff effs unit :=
+  send \o Put.
+
+Definition modify {s effs} `{Member (State s) effs} (f : s -> s) : Eff effs unit :=
+  fmap f get >>= put.
+
+Definition gets {s a effs} `{Member (State s) effs} (f : s -> a) : Eff effs a :=
+  f <$> get.
+
+Definition stateAlg {s : Type} `(f : State s a) (st : s) : a * s :=
+  match f with
+  | Get   => (st, st)
+  | Put s => (tt, s)
+  end.
+
+Definition runState {s r a} (st : s) : Eff (State s :: r) a -> Eff r (a * s) :=
+  handleRelayS st (fun s x => Pure (x, s))
+    (fun _ s x k => let '(a, s') := stateAlg x s in k s' a).
+
+(************************************************************************)
+
+Require Import Hask.Control.Lens.
+
+Definition readonly `(l : Lens' s r) {effs} :
+  Eff (Reader r :: effs) ~> Eff (State s :: effs) :=
+  reinterpret (fun _ f =>
+    s <- get ;
+    pure (readerAlg (view l s) f)).
+
+Definition focus `(l : Lens' s s') {effs} :
+  Eff (State s' :: effs) ~> Eff (State s :: effs) :=
+  reinterpret (fun _ f =>
+    s' <- get ;
+    let '(a, t) := stateAlg f (view l s') in
+    put (set l t s') ;;
+    pure a).
+
+Definition appendonly `(l : Lens' s w) `{Monoid w} {effs} :
+  Eff (Writer w :: effs) ~> Eff (State s :: effs) :=
+  reinterpret (fun _ f =>
+    let '(a, w) := writerAlg f in
+    modify (over l (mappend w)) ;;
+    pure a).
+
+Definition overM `(l : Lens s t a b) `{Functor f} : (a -> f b) -> s -> f t := l f _.
+Notation "l %%~ f" := (overM l f) (at level 40).
+
+Polymorphic Inductive Foo : Type := mkFoo.
+Polymorphic Inductive Bar : Type := mkBar.
+Polymorphic Inductive Baz : Type := mkBaz.
+
+Record SomeState : Type := {
+  _foo : Foo;
+  _bar : Bar;
+  _baz : Baz;
+}.
+
+Definition foo : Lens' SomeState Foo :=
+  fun _ _ f env =>
+    f (_foo env) <&> fun g =>
+      {| _foo := g
+       ; _bar := _bar env
+       ; _baz := _baz env |}.
+
+Definition bar : Lens' SomeState Bar :=
+  fun _ _ f env =>
+    f (_bar env) <&> fun g =>
+      {| _foo := _foo env
+       ; _bar := g
+       ; _baz := _baz env |}.
+
+Definition baz : Lens' SomeState Baz :=
+  fun _ _ f env =>
+    f (_baz env) <&> fun g =>
+      {| _foo := _foo env
+       ; _bar := _bar env
+       ; _baz := g |}.
+
+#[local]
+Declare Instance Baz_Monoid : Monoid Baz.
+
+Definition sample {effs} :
+  Eff (Reader Foo :: State Bar :: Writer Baz :: effs) unit :=
+  Pure tt.
+
+Definition example : Eff [State SomeState] unit :=
+  subsume _
+    (focus baz _
+        (appendonly (fun _ _ => id) _
+           (subsume _
+              (focus bar _
+                 (subsume _
+                    (focus foo _
+                       (readonly (fun _ _ => id) _ sample))))))).
