src/Effects/Union.v
@@ -1,0 +1,73 @@
+Require Import
+  Coq.Lists.List.
+
+Import ListNotations.
+
+Generalizable All Variables.
+Set Primitive Projections.
+
+Inductive UnionF (a : Type) : list (Type -> Type) -> Type :=
+  | UThis : forall t r, t a -> UnionF a (t :: r)
+  | UThat : forall t r, UnionF a r -> UnionF a (t :: r).
+
+Arguments UThis {a t r} _.
+Arguments UThat {a t r} _.
+
+Definition Union (r : list (Type -> Type)) (a : Type) : Type := UnionF a r.
+
+Lemma Union_empty : forall a, Union [] a -> False.
+Proof. inversion 1. Qed.
+
+(* A notation for natural transformations. *)
+Notation "f ~> g" := (forall x, f x -> g x) (at level 90).
+
+Import EqNotations.
+
+Program Definition decomp `(u : Union (t :: r) v) : t v + Union r v :=
+  match u in UnionF _ xs
+        return (t :: r)%list = xs -> t v + Union r v with
+  | UThis x => fun _ => inl (_ x)
+  | UThat x => fun _ => inr x
+  end eq_refl.
+
+Definition decomp_rev `(u : Union (r ++ [t]) v) : Union r v + t v.
+Proof.
+  induction r; simpl in u.
+    inversion u; subst.
+      exact (inr X).
+    inversion X.
+  inversion u; subst.
+    exact (inl (UThis X)).
+  destruct (IHr X).
+    exact (inl (UThat u0)).
+  exact (inr t0).
+Defined.
+
+Program Definition extract `(u : Union [t] v) : t v :=
+  match decomp u with | inl x => x | inr x => False_rect _ _ end.
+Next Obligation. inversion x. Qed.
+
+Definition weaken {any} `(u : Union r v) : Union (any :: r) v := UThat u.
+
+Fixpoint inject_last  (t : Type -> Type) (r : list (Type -> Type))
+         `(x : t a) : Union (r ++ [t]) a :=
+  match r with
+  | [] => UThis x
+  | _ :: xs => UThat (inject_last t xs x)
+  end.
+
+Class Weakens q := {
+  weakens {r a} : Union r a -> Union (q ++ r) a
+}.
+
+Import ListNotations.
+
+#[export]
+Program Instance nil_Weakens : Weakens [] := {|
+  weakens := fun _ _ => id
+|}.
+
+#[export]
+Program Instance cons_Weakens {x xs} `{Weakens xs} : Weakens (x :: xs) := {|
+  weakens := fun _ _ u => weaken (weakens u)
+|}.
